[riscv] WIP RunningExample.v for TotalBlockVer, exclude from _CoqProject for now

case_study/RiscvPmp/TotalBlockVer/RunningExample.v
@@ -40,7 +40,10 @@ From Katamaran Require Import
      RiscvPmp.BlockVer.Spec
      RiscvPmp.BlockVer.Verifier
      RiscvPmp.Machine
-     RiscvPmp.Sig.
+     RiscvPmp.Sig
+     RiscvPmp.IrisModelBinary
+     RiscvPmp.IrisInstanceBinary
+     RiscvPmp.ModelBinary.
 
 Import RiscvPmpProgram.
 Import RiscvPmpBlockVerifExecutor.
@@ -81,9 +84,17 @@ Section Utils.
   Section WithAsnNotations.
     Import AsnNotations.
 
-    Definition pmp_cfg {Σ} : Term Σ (ty.list (ty.prod ty_pmpcfg_ent ty_xlenbits)) := 
-      term_list [(term_val ty_pmpcfg_ent default_pmpcfg_ent ,ₜ term_val ty_xlenbits bv.zero);
-                 (term_val ty_pmpcfg_ent default_pmpcfg_ent ,ₜ term_val ty_xlenbits bv.zero)].
+    Definition pmp_cfg : list PmpCheck.PmpEntryCfg :=
+      [(default_pmpcfg_ent , bv.zero); (default_pmpcfg_ent , bv.zero)].
+
+    (* TODO: port this into something shared so femto can reuse this (without needing to specify this kind of stuff once as a term, and once as a list! *)
+    Definition pmp_cfg_to_term {Σ} : list PmpCheck.PmpEntryCfg -> list (Term Σ (ty.prod ty_pmpcfg_ent ty_xlenbits)) :=
+      let term_cfg cfg := term_val ty_pmpcfg_ent cfg in
+      let term_addr a  := term_val ty_xlenbits a in
+      map (fun '(cfg , addr) => term_binop bop.pair (term_cfg cfg) (term_addr addr)).
+
+    Definition term_pmp_cfg {Σ} : Term Σ (ty.list (ty.prod ty_pmpcfg_ent ty_xlenbits)) :=
+      term_list (pmp_cfg_to_term pmp_cfg).
   End WithAsnNotations.
 End Utils.
 
@@ -110,7 +121,7 @@ Module UnaryCheck.
       mepc ↦ term_val ty_xlenbits (bv.of_N adv_addr) ∗
       cur_privilege ↦ term_val ty_privilege Machine ∗
       asn_regs_ptsto ∗
-      asn_pmp_entries pmp_cfg.
+      asn_pmp_entries term_pmp_cfg.
 
     Definition POST : AssertionWith ["a" :: ty_xlenbits; "an" :: ty_xlenbits] :=
       (term_var "an" = term_val ty_xlenbits (bv.of_N adv_addr))%asn ∗
@@ -120,7 +131,7 @@ Module UnaryCheck.
       (∃ "v", mepc ↦ term_var "v") ∗
       cur_privilege ↦ term_val ty_privilege User ∗
       asn_regs_ptsto ∗
-      asn_pmp_entries pmp_cfg.
+      asn_pmp_entries term_pmp_cfg.
   End WithAsnNotations.
 
   Definition vc_code : 𝕊 ε :=
@@ -141,5 +152,84 @@ Module RunningExample.
   (* First version of the running example is the bare minimum, just making sure
      that all the building blocks fit together. The example is a MRET instr,
      with the entire memory and all registers public (i.e., there are no secrets). *)
+
+  (* Reuse the existing PRE and POST defined in UnaryCheck (doesn't specify
+     which logic to use for the block verifier, so this should be fine). *)
+  Definition PRE := UnaryCheck.PRE.
+  Definition POST := UnaryCheck.POST.
+
+  Definition vc_code : 𝕊 ε :=
+    postprocess (TotalBlockVer.Verifier.sblock_verification_condition PRE code POST wnil).
+
+  Lemma sat_code : TotalBlockVer.Verifier.safeE vc_code.
+  Proof.
+    vm_compute.
+    constructor; cbn.
+    intuition; bv_solve_Ltac.solveBvManual.
+  Qed.
+
+  Section WithIris.
+    Import iris.program_logic.weakestpre.
+    Import iris.proofmode.tactics.
+    Import RiscvPmpIrisBase2.
+    Import RiscvPmpIrisInstance2.
+
+    #[local] Notation "a '↦ᵣ' t" := (reg_pointsTo2 a t t).
+
+    (* Ref: femto_handler_pre *)
+    Definition iPRE `{sailGS2 Σ} : iProp Σ :=
+      mstatus ↦ᵣ {| MPP := User |} ∗
+      (∃ v, mtvec ↦ᵣ v) ∗
+      (∃ v, mcause ↦ᵣ v) ∗
+      mepc ↦ᵣ (bv.of_N adv_addr) ∗
+      cur_privilege ↦ᵣ Machine ∗
+      interp_gprs ∗
+      interp_pmp_entries pmp_cfg.
+
+    Definition iPOST `{sailGS2 Σ} : iProp Σ :=
+      (∃ v, mstatus ↦ᵣ v) ∗
+      (∃ v, mtvec ↦ᵣ v) ∗
+      (∃ v, mcause ↦ᵣ v) ∗
+      (∃ v, mepc ↦ᵣ v) ∗
+      cur_privilege ↦ᵣ User ∗
+      interp_gprs ∗
+      interp_pmp_entries pmp_cfg.
+
+    Import IrisInstance.RiscvPmpIrisInstance.
+    Print WP2_loop.
+    Definition contract `{sailGS2 Σ} : iProp Σ :=
+      semTTriple [env] iPRE fun_step (λ _ _, iPOST).
+
+    Definition contract `{sailGS2 Σ} : iProp Σ :=
+      iPRE -∗
+        (iPOST -∗ WP2_loop) -∗
+          WP2_loop.
+
+    Lemma contract_verified : ∀ `{sailGS2 Σ}, ⊢ contract.
+    Proof.
+      iIntros (Σ sG) "Hpre Hk".
+      iDestruct "Hpre" as "((Hmstatus₁ & Hmstatus₂) & (%mtvec & Hmtvec₁ & Hmtvec₂)
+                          & (%mcause & Hmcause₁ & Hmcause₂) & (Hmepc₁ & Hmepc₂)
+                          & (Hcp₁ & Hcp₂) & Hgprs & Hpmp)".
+      iPoseProof (RiscvPmpModel2.interp_pmpentries_dedup with "Hpmp") as "(Hpmp₁ & Hpmp₂)".
+      iPoseProof (RiscvPmpModel2.interp_gprs_split with "Hgprs") as "(Hgprs₁ & Hgprs₂)".
+      iApply semWP2_focus.
+
+      
+      iApply semWP2_anaglyph.
+      iApply (semWP_mono with "[-]").
+      - iApply (sound_sblock_verification_condition with "[-Hk Hmstatus₂ Hmtvec₂ Hmcause₂ Hmepc₂ Hcp₂ Hpmp₂ Hgprs₂] [Hk Hmstatus₂ Hmtvec₂ Hmcause₂ Hmepc₂ Hcp₂ Hpmp₂ Hgprs₂]").
+        + apply UnaryCheck.sat_code.
+        + cbn - [asn_regs_ptsto].
+          iPoseProof (@Model.RiscvPmpModel2.gprs_equiv _ RiscvPmpModel2.sailGS2_sailGS_left with "Hgprs₁") as "Hgprs₁".
+          iFrame "Hmstatus₁ Hmtvec₁ Hmcause₁ Hmepc₁ Hcp₁ Hpmp₁ Hgprs₁".
+          admit (* TODO: missing some stuff in the pre and post above :) *).
+        + cbn.
+          iIntros (an) "(Hpc₁ & Hnpc₁ & Hhandler & H & Hmstatus₁ & Hmtvec₁ & Hmcause₁ & Hmepc₁ & Hcurpriv₁ & Hregs₁ & Hpmp₁)".
+          unfold iPOST.
+          iSpecialize ("Hk" with "[$Hmstatus]").
+      -
+
+  End WithIris.
 
 End RunningExample.
